

CSE260

Digital Logical Design

Name: Tahmina Rahman Fecha

ID: 23201429

Section: 06(B)

Faculty: Dewan Ziaul Karim (DZK)

Assignment - 02

Date: 06.11.2025

Ans no 1

$$(A \oplus B)(C+D)(A \odot C) + (A+B)(C'+D)(A'+CC') \quad \text{--- ①}$$

Here, $A \oplus B = A'B + AB'$

$$A \odot C = AC + A'C'$$

Now ① \Rightarrow

$$(A'B + AB')(C+D)(AC + A'C') + (A+B)(C'+D)(A' + CC')$$

$$CC' = 0 ; A' + CC' = A'$$

① \Rightarrow

$$\begin{aligned} & (A'B + AB')(C+D)(AC + A'C') + (A+B)(C'+D)(A') \\ &= (A'BC + A'BD + AB'C + AB'D)(AC + A'C') + (AC' + AD + BC' + BD)(A') \\ &= (AA'BC + A'BC C' + AA'BCD + A'BC'D + AB'C + AA'B'CC' + AB'CD + AA'B'CD) \\ & \quad + (AA'C' + AA'D + A'BC' + A'BD) \\ &= (A'BC'D + AB'C + AB'CD) + (A'BC' + A'BD) \quad [\because AA' = 0 \text{ \& } ACC' = 0] \\ &= A'BC'D + AB'C(1+D) + A'BC' + A'BD \\ &= A'BC'D + AB'C + A'BC + A'BD \\ &= A'B(C+D+C'D) + AB'C \end{aligned}$$

Ans no 2

$$F = (x' + y + z')(x + y')(x' + z)$$

Using DeMorgan's Law, Theorem,

$$F' = [(x' + y + z')(x + y')(x' + z)]'$$

$$\Rightarrow F' = (x' + y + z')' + (x + y')' + (x' + z)' \quad [\because (AB)' = A' + B']$$

$$\Rightarrow F' = ((x')' \cdot y' \cdot (z')') + (x' \cdot (y')') + ((x')' \cdot z') \quad [\because (A+B)' = A'B']$$

$$\Rightarrow F' = xy'z + x'y + xz'$$

$$\Rightarrow F' = x(y'z + z') + x'y$$

$$\Rightarrow F' = x(y' + z')(z + z') + x'y$$

$$\Rightarrow F' = x(y' + z') + x'y \quad [\because z + z' = 1]$$

$$\Rightarrow F' = xy' + xz' + x'y$$

SOP

Ans no 3

consensus theorem,

$$AB + A'C + BC = AB + A'C$$

Comparing with $F = WY + WX + X'Y$,

$$AB = WX, A'C = X'Y, BC = WY$$

~~By consensus theorem,~~

$$F(V, W, X, Y, Z) = WY + WX + X'Y$$

$$= WY[(V+V')(X+X')(Z+Z')] + WX[(V+V')(Y+Y')(Z+Z')] + X'Y[(V+V')(W+W')(Z+Z')]$$

$$= WY(WXZ + VXZ' + VX'Z + VX'Z' + V'XZ + V'X'Z + V'XZ' + V'X'Z') + WX(VYZ + VYZ' + V'YZ + V'YZ' + VY'Z + VY'Z' + V'Y'Z + V'Y'Z') + X'Y(VWZ + VWZ' + V'WZ + V'WZ' + VW'Z + VW'Z' + V'W'Z + V'W'Z')$$

$$= VWXYZ + VWXYZ' + VWX'YZ + VWX'YZ' + V'WXYZ + V'WX'YZ + V'WXYZ' + V'WX'YZ' + VWXY'Z + VWXY'Z' + V'WX'YZ + V'WX'YZ' + VWX'Y'Z + VWX'Y'Z' + V'WX'Y'Z + V'WX'Y'Z' + VW'XYZ + VW'XYZ' + V'W'XYZ + V'W'XYZ' \\ = VWXYZ + VWXYZ' + VWXY'Z + VWX'YZ + VWX'YZ' \quad (P.T.O)$$

$$\begin{aligned}
 &+ VWXY'Z' + V'WX'YZ + V'WX'YZ' + V'WX'YZ + V'WX'YZ' \\
 &+ V'WX'YZ' + V'WX'YZ' + VW'X'YZ + VW'X'YZ' \\
 &+ V'WX'YZ + V'WX'YZ'
 \end{aligned}$$

(Total 16 minterms) Ans.

POS Using consensus theorem,

$$F = WX + X'Y \quad [\because AB + A'C + BC = AB + A'C; \\
 AB = WX, A'C = X'Y]$$

Using distributive law $(A + BC) = (A + B)(A + C)$:

$$\begin{aligned}
 F &= (WX + X')(WX + Y) \\
 &= (W + X')(X + X')(W + Y)(X + Y) [A + BC = (A + B)(A + C)] \\
 &= (W + X')(W + Y)(X + Y) \\
 &= (W + X' + VV')(W + Y + VV')(X + Y + VV') [Adding V] \\
 &= (W + X' + V)(W + X' + V')(W + Y + V)(W + Y + V')(X + Y + V)(X + Y + V') \\
 &= (W + X' + V + YY')(W + X' + V' + YY')(W + Y + V + XX')(W + Y + V' + XX') \\
 &\quad (X + Y + V + WW')(X + Y + V' + WW') [Adding W, Y] \\
 &= (W + X' + V + Y)(W + X' + V + Y')(W + X' + V' + Y)(W + X' + V' + Y') \\
 &\quad (W + Y + V + X)(W + Y + V + X')(W + Y + V' + X)(W + Y + V' + X') \\
 &\quad (X + Y + V + W)(X + Y + V + W')(X + Y + V' + W)(X + Y + V' + W')
 \end{aligned}$$

(P.T.O)

$$\begin{aligned}
&= (w+x'+v+y+zz')(w+x'+v+y'+zz')(w+x'+v'+y+zz') \\
&\quad (w+x'+v'+y'+zz')(w+y+v+x+zz')(w+y+v+x'+zz') \\
&\quad (w+y+v'+x+zz')(w+y+v'+x'+zz')(x+y+v+w+zz') \\
&\quad (x+y+v+w'+zz')(x+y+v'+w+zz')(x+y+v'+w'+zz') \\
&\hspace{15em} [\text{Adding } z]
\end{aligned}$$

$$\begin{aligned}
&\stackrel{2}{=} (w+x'+v+y+z)(w+x'+v+y+z')(w+x'+v+y'+z)(w+x'+v+y'+z') \\
&\quad (w+x'+v'+y+z)(w+x'+v'+y+z')(w+x'+v'+y'+z)(w+x'+v'+y'+z') \\
&\quad (w+y+v+x+z)(w+y+v+x+z')(w+y+v+x'+z)(w+y+v+x'+z') \\
&\quad (w+y+v'+x+z)(w+y+v'+x'+z')(w+y+v'+x'+z)(w+y+v'+x'+z') \\
&\quad (x+y+v+w+z)(x+y+v+w+z')(x+y+v+w'+z)(x+y+v+w'+z') \\
&\quad (x+y+v'+w+z)(x+y+v'+w+z')(x+y+v'+w'+z)(x+y+v'+w'+z')
\end{aligned}$$